PropositionalLogic/Sound_Kripke.v
@@ -1,0 +1,216 @@
+Require Import Coq.Classes.RelationClasses.
+Require Import Coq.Relations.Relation_Definitions.
+Require Import Logic.LogicBase.
+Require Import Logic.MinimunLogic.MinimunLogic.
+Require Import Logic.MinimunLogic.ContextProperty.
+Require Import Logic.PropositionalLogic.Syntax.
+Require Import Logic.PropositionalLogic.KripkeSemantics.
+Require Import Logic.PropositionalLogic.IntuitionisticPropositionalLogic.
+Require Import Logic.PropositionalLogic.ClassicalPropositionalLogic.
+
+Local Open Scope logic_base.
+Local Open Scope PropositionalLogic.
+
+Lemma sound_modus_ponens {L: Language} {nL: NormalLanguage L} {pL: PropositionalLanguage L} {SM: Semantics L} {pkS: PreKripkeSemantics L SM} {kiSM: KripkeIntuitionisticSemantics L SM}:
+  forall x y: expr,
+    forall M m,
+      KRIPKE: M, m |= (x --> y) -> KRIPKE: M, m |= x -> KRIPKE: M, m |= y.
+Proof.
+  intros.
+  pose proof Korder_PreOrder M as H_PreOrder.
+  rewrite sat_impp in H.
+  specialize (H m).
+  apply H; auto.
+  reflexivity.
+Qed.
+
+Lemma sound_axiom1 {L: Language} {nL: NormalLanguage L} {pL: PropositionalLanguage L} {SM: Semantics L} {pkS: PreKripkeSemantics L SM} {kiSM: KripkeIntuitionisticSemantics L SM}:
+  forall x y: expr,
+    forall M m,
+      KRIPKE: M, m |= x --> y --> x.
+Proof.
+  intros.
+  rewrite sat_impp; intros.
+  rewrite sat_impp; intros.
+  eapply sat_mono; eauto.
+Qed.
+
+Lemma sound_axiom2 {L: Language} {nL: NormalLanguage L} {pL: PropositionalLanguage L} {SM: Semantics L} {pkS: PreKripkeSemantics L SM} {kiSM: KripkeIntuitionisticSemantics L SM}:
+  forall x y z: expr,
+    forall M m,
+      KRIPKE: M, m |= (x --> y --> z) --> (x --> y) --> (x --> z).
+Proof.
+  intros.
+  pose proof Korder_PreOrder M as H_PreOrder.
+  rewrite sat_impp; intros.
+  rewrite sat_impp; intros.
+  rewrite sat_impp; intros.
+  assert (Korder n1 n) by (etransitivity; eauto).
+
+  rewrite sat_impp in H0.
+  specialize (H0 n1 H5 H4).
+  rewrite sat_impp in H2.
+  specialize (H2 n1 H3 H4).
+
+  assert (Korder n1 n1) by reflexivity.
+  rewrite sat_impp in H0.
+  specialize (H0 n1 H6 H2).
+  auto.
+Qed.
+
+Lemma sound_andp_intros {L: Language} {nL: NormalLanguage L} {pL: PropositionalLanguage L} {SM: Semantics L} {pkS: PreKripkeSemantics L SM} {kiSM: KripkeIntuitionisticSemantics L SM}:
+  forall x y: expr,
+    forall M m,
+      KRIPKE: M, m |= x --> y --> x && y.
+Proof.
+  intros.
+  rewrite sat_impp; intros.
+  rewrite sat_impp; intros.
+  rewrite sat_andp.
+  split.
+  + eapply sat_mono; eauto.
+  + auto.
+Qed.
+
+Lemma sound_andp_elim1 {L: Language} {nL: NormalLanguage L} {pL: PropositionalLanguage L} {SM: Semantics L} {pkS: PreKripkeSemantics L SM} {kiSM: KripkeIntuitionisticSemantics L SM}:
+  forall x y: expr,
+    forall M m,
+      KRIPKE: M, m |= x && y --> x.
+Proof.
+  intros.
+  rewrite sat_impp; intros.
+  rewrite sat_andp in H0.
+  tauto.
+Qed.
+
+Lemma sound_andp_elim2 {L: Language} {nL: NormalLanguage L} {pL: PropositionalLanguage L} {SM: Semantics L} {pkS: PreKripkeSemantics L SM} {kiSM: KripkeIntuitionisticSemantics L SM}:
+  forall x y: expr,
+    forall M m,
+      KRIPKE: M, m |= x && y --> y.
+Proof.
+  intros.
+  rewrite sat_impp; intros.
+  rewrite sat_andp in H0.
+  tauto.
+Qed.
+
+Lemma sound_orp_intros1 {L: Language} {nL: NormalLanguage L} {pL: PropositionalLanguage L} {SM: Semantics L} {pkS: PreKripkeSemantics L SM} {kiSM: KripkeIntuitionisticSemantics L SM}:
+  forall x y: expr,
+    forall M m,
+      KRIPKE: M, m |= x --> x || y.
+Proof.
+  intros.
+  rewrite sat_impp; intros.
+  rewrite sat_orp.
+  tauto.
+Qed.
+
+Lemma sound_orp_intros2 {L: Language} {nL: NormalLanguage L} {pL: PropositionalLanguage L} {SM: Semantics L} {pkS: PreKripkeSemantics L SM} {kiSM: KripkeIntuitionisticSemantics L SM}:
+  forall x y: expr,
+    forall M m,
+      KRIPKE: M, m |= y --> x || y.
+Proof.
+  intros.
+  rewrite sat_impp; intros.
+  rewrite sat_orp.
+  tauto.
+Qed.
+
+Lemma sound_orp_elim {L: Language} {nL: NormalLanguage L} {pL: PropositionalLanguage L} {SM: Semantics L} {pkS: PreKripkeSemantics L SM} {kiSM: KripkeIntuitionisticSemantics L SM}:
+  forall x y z: expr,
+    forall M m,
+      KRIPKE: M, m |= (x --> z) --> (y --> z) --> (x || y --> z).
+Proof.
+  intros.
+  pose proof Korder_PreOrder M as H_PreOrder.
+  rewrite sat_impp; intros.
+  rewrite sat_impp; intros.
+  rewrite sat_impp; intros.
+  rewrite sat_orp in H4.
+  destruct H4.
+  + rewrite sat_impp in H0.
+    apply H0; auto.
+    etransitivity; eauto.
+  + rewrite sat_impp in H2.
+    apply H2; auto.
+Qed.
+
+Lemma sound_falsep_elim {L: Language} {nL: NormalLanguage L} {pL: PropositionalLanguage L} {SM: Semantics L} {pkS: PreKripkeSemantics L SM} {kiSM: KripkeIntuitionisticSemantics L SM}:
+  forall x: expr,
+    forall M m,
+      KRIPKE: M, m |= FF --> x.
+Proof.
+  intros.
+  rewrite sat_impp; intros.
+  pose proof sat_falsep M n.
+  tauto.
+Qed.
+
+Lemma sound_excluded_middle_ident {L: Language} {nL: NormalLanguage L} {pL: PropositionalLanguage L} {SM: Semantics L} {pkS: PreKripkeSemantics L SM} {kiSM: KripkeIntuitionisticSemantics L SM}:
+  forall x: expr,
+    forall M,
+      (forall m n, @Korder _ _ _ _ _ _ M m n -> m = n) ->
+      (forall m, KRIPKE: M, m |= x || ~~ x).
+Proof.
+  intros.
+  unfold negp.
+  rewrite sat_orp, sat_impp.
+  destruct (Classical_Prop.classic (KRIPKE: M, m |= x)); auto.
+  right; intros.
+  apply H in H1; subst n.
+  tauto.
+Qed.
+
+Theorem sound_intuitionistic_kripke_all (Var: Type): sound (IntuitionisticPropositionalLogic.G Var) (KripkeSemantics_All.SM Var).
+Proof.
+  hnf; intros.
+  pose (KripkeSemantics_All.SM Var) as SM.
+  pose (KripkeSemantics_All.pkSM Var) as pkSM.
+  pose (KripkeSemantics_All.kiSM Var) as kiSM.
+  intro m.
+  destruct m as [M m].
+  change (@Kmodel _ _ pkSM) in M.
+  change (Kworlds M) in m.
+  change (KRIPKE: M, m |= x).
+  induction H.
+  + pose proof sound_modus_ponens x y M m.
+    exact (H1 IHprovable1 IHprovable2).
+  + apply sound_axiom1.
+  + apply sound_axiom2.
+  + apply sound_andp_intros.
+  + apply sound_andp_elim1. 
+  + apply sound_andp_elim2.
+  + apply sound_orp_intros1.
+  + apply sound_orp_intros2.
+  + apply sound_orp_elim.
+  + apply sound_falsep_elim.
+Qed.
+
+Theorem sound_classical_kripke_identical (Var: Type): sound (ClassicalPropositionalLogic.G Var) (KripkeSemantics_Identical.SM Var).
+Proof.
+  hnf; intros.
+  pose (KripkeSemantics_Identical.SM Var) as SM.
+  pose (KripkeSemantics_Identical.pkSM Var) as pkSM.
+  pose (KripkeSemantics_Identical.kiSM Var) as kiSM.
+  intro m.
+  destruct m as [M m].
+  change (@Kmodel _ _ pkSM) in M.
+  change (Kworlds M) in m.
+  change (KRIPKE: M, m |= x).
+  induction H.
+  + pose proof sound_modus_ponens x y M m.
+    exact (H1 IHprovable1 IHprovable2).
+  + apply sound_axiom1.
+  + apply sound_axiom2.
+  + apply sound_andp_intros.
+  + apply sound_andp_elim1. 
+  + apply sound_andp_elim2.
+  + apply sound_orp_intros1.
+  + apply sound_orp_intros2.
+  + apply sound_orp_elim.
+  + apply sound_falsep_elim.
+  + apply sound_excluded_middle_ident.
+    apply (@KripkeSemantics_Identical.frame_ident Var M).
+Qed.
+
+
