Makefile
@@ -12,4 +12,4 @@ all: Wf.vo base.vo IPC.vo trivial.vo Kripke.vo enumerate.vo LogicBase.vo \
      PropositionalLogic/TrivialSemantics.vo PropositionalLogic/Sound_Classical_Trivial.vo \
      PropositionalLogic/Complete_Classical_Trivial.vo lib/Coqlib.vo \
      lib/Bijection.vo lib/Countable.vo PropositionalLogic/Complete_Intuitionistic_Kripke.vo \
-     PropositionalLogic/CanonicalKripke.vo 
+     PropositionalLogic/CanonicalKripke.vo PropositionalLogic/Sound_Kripke.vo
